theories/run_prop.v
@@ -899,7 +899,7 @@ Section RunP.
     ( runb u s0 A sm (clean_success A'') b1 /\
       (if has_bt A A'' then runb u sm B0 sn (clean_success B' ) b2
       else runb u sm B sn (clean_success B' ) b2) /\
-      A' = clean_success (if b2 == 0 then A'' else cutl A'')).
+      A' = (if b2 == 0 then A'' else cutl A'')).
   Proof.
     remember (And _ _ _) as O1 eqn:HO1.
     remember (And A' _ _) as O2 eqn:HO2.
@@ -917,7 +917,7 @@ Section RunP.
         - rewrite (expandedb_has_bt H1)//clean_success2//; apply: run_done H2 erefl.
         - move=> //.
       have := expanded_Done_success _ H1.
-      (* rewrite -success_cut => sA''.
+      rewrite -success_cut => sA''.
       rewrite sA'' => -[???]; subst.
       repeat eexists.
       - apply: run_done H1 erefl.
@@ -970,14 +970,14 @@ Section RunP.
         have {IH} := IH _ _ _ _ _ _ erefl erefl.
         move=>[A''[b3[b4[sm [rE2 [+ H6]]]]]]; subst.
         have [[? H ]?] := run_consistent _ rE2 (runb_success _ _ sA'''); subst.
-        have:= clean_success_cutl _ sA'''.
-        rewrite cutl2 -H => Hw.
+        (* have:= clean_success_cutl _ sA'''. *)
+        (* rewrite cutl2 -H => Hw. *)
         admit.
       have {IH} := IH _ _ _ _ _ _ erefl erefl.
       move=>[A''[b3[b4[sm [rE2 [+ H6]]]]]]; subst.
       have /= := is_ko_runb _ _ rE2.
       rewrite success_cut in sA'''.
-      move=> /(_ (clean_success_cutl _ sA'''))//. *)
+      (* move=> /(_ (clean_success_cutl _ sA'''))//. *)
   Admitted.
 
   (* Lemma run_and_correct_success_left {s0 sn A B B0 C b}:
